\documentclass[12pt, a4paper]{amsart}
\usepackage{amscd, amsfonts, amssymb}

\newtheorem{prop}{Proposition}
\newtheorem{defn}{Definition}

\usepackage{parskip}

\usepackage{mathrsfs}
\usepackage[all]{xy}

%\usepackage[landscape]{geometry}

\begin{document}

\title{Maps of 1-Cohomologies}
\maketitle
\begin{prop}
	Let $f:K'\rightarrow K$, $K'$ an algebraic group also acting on $V$ by group automorphisms. Then $\alpha \circ f$ is a 1-cocycle from $K' \rightarrow V$.
\end{prop}
\begin{proof}
\end{proof}

The map $\zeta:Z^1(K, V) \rightarrow Z^1(K', V)$ defined by
\begin{eqnarray*}
	\zeta(\alpha) &=& \alpha \circ f
\end{eqnarray*}
is a map of 1-cocycles.

\begin{prop}
	Let $g:V \rightarrow V'$ be an equivariant homomorphism. Then $g \circ \alpha$ is a 1-cocycle from $K \rightarrow V'$.
\end{prop}
\begin{proof}
\end{proof}

The map $\xi:Z^1(K, V) \rightarrow Z^1(K, V')$ defined by
\begin{eqnarray*}
	\xi(\alpha) = g \circ \alpha
\end{eqnarray*}
is a map of 1-cocycles. More generally, we have the following Definition.

\begin{defn}
	Define the map
	\begin{eqnarray*}
		Z^1(\zeta, \xi):Z^1(K, V) \rightarrow Z^1(K', V')
	\end{eqnarray*}
	by
	\begin{eqnarray*}
		Z^1(\zeta, \xi)(\alpha) = g \circ \alpha \circ f.
	\end{eqnarray*}
\end{defn}

Then, for example,
\begin{eqnarray*}
	Z^1(\zeta, \mathrm{id}) = \zeta, && \textrm{where }\mathrm{id}:V\rightarrow V \textrm{ is the identity map, and} \\
	Z^1(\mathrm{id}, \xi) = \xi,     && \textrm{where }\mathrm{id}:H\rightarrow H \textrm{ is the identity map}.
\end{eqnarray*}


\begin{prop}
	The map $Z^1(\zeta, \xi)$ descends to give a well-defined map
	\begin{eqnarray*}
		H^1(\zeta, \xi):H^1(K, V) \rightarrow H^1(K', V')
	\end{eqnarray*}
	of 1-cohomologies, defined by
	\begin{eqnarray*}
		H^1(\zeta, \xi)\left(\psi(\alpha)\right) = \left(\psi' \circ Z^1(\zeta, \xi)\right)(\alpha),
	\end{eqnarray*}
	where $\psi:Z^1(K, V)\rightarrow H^1(K, V)$ and $\psi':Z^1(K', V')\rightarrow H^1(K, V)$ are the canonical projections. Moreover, the following diagram commutes.
	\begin{eqnarray*}
	\xymatrix{
	Z^1(K, V) \ar[d]_{\psi} \ar[r]^{Z^1(\zeta, \xi)} & Z^1(K', V') \ar[d]^{\psi'} \\
	H^1(K, V)               \ar[r]^{H^1(\zeta, \xi)} & H^1(K', V') \\
	}
	\end{eqnarray*}
\end{prop}
\begin{proof}
\end{proof}
\end{document}
