%!TEX root = ../Thesis.tex
% Chapter 3

\chapter{The 1-Cohomology}
\label{Chapter3}
\lhead{Chapter 3. \emph{The 1-Cohomology}}

\section{Abelian 1-Cohomology}
The abelian 1-cohomology is standard (cf. \cite{brown1976cohomology}). We present this Section as motivation for the less-known non-abelian theory to appear in the next Section.

Let $K$ be an algebraic group and $V$ an abelian group on which $K$ acts by group automorphisms. We denote the action by $x \cdot v$, for $x \in K, v \in V$.

\begin{definition} We call a morphism $\alpha$ from $K\rightarrow V$ a \emph{1-cocycle} if it satisfies
	\begin{align}
		\alpha(xy) = \alpha(x) + x\cdot\alpha(y),
		\label{eqn:a_z}
	\end{align}
	for all $x, y$ in $K$. Denote by $Z^1\left( K, V \right)$ the collection of all 1-cocycles from $K\rightarrow V$.

	We call Equation \ref{eqn:a_z} the \emph{1-cocycle condition}.
\end{definition}

For any $\alpha, \beta$ in $Z^1\left(K, V\right)$,
\begin{align*}
	\left(\alpha + \beta\right)(xy) &=  \alpha(xy) +  \beta(xy) \\
	&=  \alpha(x) + x\cdot\alpha(y) +  \beta(x) + x\cdot\beta(y)\\
	&=  \left( \alpha(x) + \beta(x) \right) + x\cdot\left(\alpha(y) + \beta(y)\right) \\
	&=  \left(\alpha+\beta\right)(x) + x\cdot\left(\alpha + \beta\right)(y).
\end{align*}
It is easy to check that $\alpha + \beta$ is a morphism, so $Z^1(K, V)$ is closed under pointwise addition.

The trivial map from $K \rightarrow V$ that sends every $h \in K$ to the identity $0 \in V$ is a 1-cocycle. Furthermore for any $\alpha \in Z^1(K, V)$ we have
\begin{align*}
	\alpha(1)\, =\, \alpha(1\cdot 1) &=  \alpha(1) + 1\cdot \alpha(1) \\
	&=  \alpha(1) + \alpha(1) \\
	&=  2\,\alpha(1),
\end{align*}
so $\alpha(1) = 0$. Then, for all $x \in K$,
\begin{align*}
	0 = \alpha(1) = \alpha(xx^{-1}) = \alpha(x) + x \cdot \alpha(x^{-1})
\end{align*}
Hence each $\alpha$ has a negative defined by
\begin{align*}
	-\alpha(x) = x\cdot\alpha(x^{-1}).
\end{align*}
Therefore $Z^1\left(K, V\right)$ is an abelian $\mathbb{Z}-$module under pointwise addition.

\begin{definition} Let $v \in V$. The morphism $\chi^K_v:K\rightarrow V$ defined by
\begin{align*}
	\chi^K_v (x) = v - x\cdot v,
\end{align*}
is called a \emph{1-coboundary}. We denote by $B^1\left(K, V\right)$ the collection of all 1-coboundaries. 
\end{definition}

For any $v \in V$ and any $x, y \in K$
\begin{align*}
	\chi^K_v(xy) &=  v - (xy)\cdot v \\
	&=  v - x \cdot \left(y\cdot v \right)\\
	&=  v - x \cdot \left(v -v + y\cdot v \right)\\
	&=  v - x\cdot v + x\cdot \left( v - y\cdot v\right)\\
	&=  \chi^K_v(x) + x\cdot \chi^K_v(y),
\end{align*}
so $B^1(K, V) \subset Z^1(K, V)$. 

For any $u,v \in V$ and all $h \in K$,
\begin{align*}
	(\chi^K_u + \chi^K_v)(h) &=  \chi^K_u(h) + \chi^K_v(h)\\
	&=  u - h\cdot u + v - h\cdot v \\
	&=  (u + v) - h\cdot (u + v) \\
	&=  \chi^K_{u + v} (h).
\end{align*}
Hence $B^1\left(K, V\right)$ is also closed under pointwise addition.

Evidently $B^1(K, V)$ is a subgroup of $Z^1(K, V)$. In fact $B^1(K, V)$ is a $\mathbb{Z}-$submodule of $Z^1(K, V)$, so we may form the quotient module.
\begin{definition} The \emph{1-cohomology} is the quotient module defined by
\begin{align*}
	H^1\left(K, V\right) = Z^1\left(K, V\right) / B^1\left(K, V\right).
\end{align*}
We denote by $\psi$ the canonical projection from $Z^1(K, V)\rightarrow H^1(K, V)$.
\end{definition}

TODO: $V$ is a vector space, $K$ acts linearly $\Rightarrow$ $B^1(K, V) \subset Z^1(K, V)$ are vector spaces: formula for scalar multiplication, formula for $\lambda\chi^K_V, \lambda \in k$.

We conclude this Section with a useful Lemma \cite[Proposition 1]{kemper2000characterization}.
\begin{lemma} Suppose $K$ is linearly reductive. Then $H^1(K, V)$ is trivial.
  \label{lem:lin_red_h}
\end{lemma}

\section{Non-abelian 1-Cohomology}
	
We no longer require that $V$ is abelian; henceforth $V$ is an algebraic group on which $K$ acts by group automorphisms. Much of the preceding Section is a direct analogue, for example many formulas are just rewritten in multiplicative notation.
One main difference will see is that 1-coboundaries are less useful in the non-abelian setting.

\begin{definition} We call a morphism $\alpha$ from $K\rightarrow V$ a \emph{1-cocycle} if it satisfies
\begin{align}
  \alpha(xy) = \alpha(x) (x\cdot\alpha(y)),
  \label{eqn:na_z}
\end{align}
for all $x, y \in K$. Denote by $Z^1\left( K, V \right)$ the collection of all 1-cocycles from $K\rightarrow V$.

We call Equation \ref{eqn:na_z} the \emph{1-cocycle condition}.
\end{definition}

\begin{remark} Unlike the previous Section there is no natural addition operation on $Z^1(K, V)$.
\end{remark}

\begin{definition} Let $v \in V$. The morphism $\chi^K_v:K\rightarrow V$ defined by
\begin{align*}
	\chi^K_v (h) = v (h\cdot v^{-1}),
\end{align*}
is called a \emph{1-coboundary}. We denote by $B^1\left(K, V\right)$ the collection of all 1-coboundaries.
\end{definition}

For any $v \in V$ and any $x, y \in K$,
\begin{align*}
	\chi^K_v(xy) &=  v \left((xy) \cdot v^{-1}\right) \\
	&=  v (x \cdot v^{-1}) (x \cdot v) ((xy) \cdot v^{-1}) \\
	&=  v \left(x \cdot v^{-1}\right) (x \cdot v) \left(x \cdot \left(y \cdot v^{-1}\right)\right) \\
	&=  v \left(x \cdot v^{-1}\right) \left(x \cdot v \left(y \cdot v^{-1}\right)\right) \\
	&=  \chi^K_v(x) (x \cdot \chi^K_v(y)),
\end{align*}
so $B^1(K, V) \subset Z^1(K, V)$.

In the abelian case we use the fact that we can take the quotient $Z^1(K, V)/B^1(K, V)$, as $B^1(K, V)$ is a $\mathbb{Z}$-submodule of $Z^1(K, V)$, but in the non-abelian they are just sets. Moreover, in the abelian case
\begin{align*}
	\psi(\alpha) = \psi(\beta) \Leftrightarrow \exists v \in V, \alpha = \beta + \chi^K_v.
\end{align*}
Again, this makes no sense in the non-abelian setting. Instead we have the following Definition.

\begin{definition} Define the relation $\sim$ on $Z^1(K, V)$ by
	\begin{align}
		\alpha \sim \beta \Leftrightarrow \exists v \in V, \alpha = v\beta(x)(x \cdot v^{-1}), \forall x \in K.
		\label{eqn:h_equiv}
	\end{align}
Then $\sim$ is an equivalence relation (TODO: show in appendix?).

Denote by $H^1(K, V)$ the \emph{1-cohomology}, defined to be the set of equivalence classes of $Z^1(K, V)$ under the relation in Equation \ref{eqn:h_equiv}, and denote by $\psi$ the canonical projection from $Z^1(K, V) \rightarrow H^1(K, V)$.
\end{definition}

R. Richardson \cite[Lemma 6.2.6]{richardson1982orbits} provides a result analogous to Lemma \ref{lem:lin_red_h}:
\begin{lemma}
  Suppose $K$ is linearly reductive and $V$ is unipotent. Then $H^1(K, V)$ is trivial.
  \label{lem:nonab_lin_red}
\end{lemma}

\section{Maps between 1-cohomologies}

The following results leading up to Lemma \ref{} could be stated in terms of the abelian 1-cohomology. Indeed we provide Lemma \ref{}, where $V$ is necessarily a vector space. However, for reasons of efficiency we state the following few definition-like results using multiplicative notation only.

As in the previous Section, $K, V$ are algebraic groups such that $K$ acts on $V$ by group automorphisms. We denote the action of $K$ on $V$ by $x \cdot v$, $x \in K, v \in V$.



\begin{example}
Let $\tilde{K}$ be a subgroup of $K$ and $\iota:\tilde{K}\rightarrow K$ the inclusion map. Then $\iota$ gives rise to the well-defined maps
\begin{align*}
  Z^1(\iota): Z^1(K, V) \rightarrow Z^1(\tilde{K}, V), \\
H^1(\iota):H^1(K, V)\rightarrow H^1(\tilde{K}, V).
\end{align*}
\end{example}

The next Lemma is standard \cite[Theorem 10.3]{brown1976cohomology} but we give our own proof here.
\begin{lemma}
Let $V$ be a vector space over a field of characteristic $p$. Let $\Gamma$ be a finite group and $\Gamma_p < \Gamma$ a \emph{Sylow $p$-subgroup} of $\Gamma$. The map 
\begin{align*}
H^1(\iota):H^1(\Gamma, V)\rightarrow H^1(\Gamma_p, V)
\end{align*}
is injective.
\label{lem:a_h_restriction}
\end{lemma}
\begin{proof}
Let $x$ be an element of $H^1(\Gamma, V)$ such that $\left(H^1(\iota)\right)(x) = 0$. Now choose a 1-cocycle $\alpha \in Z^1(\Gamma, V)$ such that $[\alpha] = x$, where $[\alpha]$ denotes the projection to the 1-cohomology. Kence $\left(Z^1(\iota)\right)(\alpha)$ is a 1-coboundary as $\left[\left(Z^1(\iota)\right)(\alpha)\right] = 0$. That is to say $\alpha$ restricted to $\Gamma_p$ is equal to a 1-coboundary, say $\chi_v^{\Gamma_p}$. But since $\chi_v^{\Gamma_p}$ can be trivially extended to a 1-coboundary $\chi_v^\Gamma$ from $\Gamma\rightarrow V$, and \begin{align*}
	\left[\alpha - \chi_v^\Gamma\right] = x,
\end{align*}
we could well have chosen the 1-cocycle $(\alpha - \chi_v^\Gamma)$ as a representative for $x$. Kence there is no harm in assuming that $\alpha$ is 0 when restricted to $\Gamma_p$.
Now choose a set of representatives $\gamma_1, \ldots, \gamma_l \in \Gamma$ for the coset space $\Gamma/\Gamma_p$ and set
\begin{align*}
	v^* = \sum_{i =1}^l \alpha(\gamma_i).
\end{align*}
Consider the 1-coboundary $\chi_{v^*}^\Gamma$:
\begin{align*}
	\chi_{v^*}^\Gamma(\gamma) &=  v^* - \gamma\cdot v^* \\
	&=  \sum_{i = 1}^l\alpha(\gamma_i) - \gamma\cdot \sum_{i = 1}^l\alpha(\gamma_i) \\
	&=  \sum_{i = 1}^l\alpha(\gamma_i) - \sum_{i = 1}^l \gamma\cdot \alpha(\gamma_i).
\end{align*}
By the 1-cocycle condition we have for all $\gamma \in \Gamma$
\begin{align*}
	\alpha(\gamma \gamma_i) = \alpha(\gamma) + \gamma\cdot\alpha(\gamma_i),
\end{align*}
for each $1 \leq i \leq l$. Therefore
\begin{align*}
	 \sum_{i = 1}^l\alpha(\gamma_i) - \sum_{i = 1}^l \gamma\cdot \alpha(\gamma_i) 
	&=  \sum_{i = 1}^l\alpha(\gamma_i) - \sum_{i = 1}^l \left(\alpha(\gamma\gamma_i) - \alpha(\gamma) \right)\\
	&=  \sum_{i = 1}^l\alpha(\gamma_i) - \sum_{i = 1}^l \alpha(\gamma\gamma_i) +\sum_{i = 1}^l \alpha(\gamma).
\end{align*}
The value of $\alpha$ at a fixed $\gamma$ depends only on the value of $\alpha$ at the representative $\gamma_j$ of the coset containing $\gamma$, and for two cosets $\gamma_i \Gamma_p, \gamma_j \Gamma_p$ and a fixed $\gamma \in \Gamma$
\begin{align}
  \gamma \gamma_i \Gamma_p = \gamma \gamma_j \Gamma_p \Leftrightarrow \gamma_i \Gamma_p = \gamma_j \Gamma_p,
\end{align}
so that $\{\gamma \gamma_i \,|\, 1 \leq i \leq l\}$ meets each coset in $\Gamma/\Gamma_p$ exactly once. Kence we can collapse the middle term to yield
\begin{align*}
	\chi_{v^*}^\Gamma(\gamma) 
	&=  \sum_{i = 1}^l\alpha(\gamma_i) - \sum_{i = 1}^l \alpha(\gamma\gamma_i) +\sum_{i = 1}^l \alpha(\gamma)\\
	&=  \sum_{i = 1}^l\alpha(\gamma_i) - \sum_{i = 1}^l \alpha(\gamma_i) +\sum_{i = 1}^l \alpha(\gamma) \\
	&=  l\, \alpha(\gamma).
\end{align*}
Since $\gcd([\Gamma:\Gamma_p], p) = \gcd(l,p) = 1$, $l$ has an inverse $l^{-1} = m$ and so
\begin{align*}
	m\chi_{v^*}^\Gamma(\gamma) = \alpha(\gamma).
\end{align*}
Therefore $\alpha$ is the 1-coboundary
\begin{align}
  m\chi_{v^*}^\Gamma = \chi_{mv^*}^\Gamma
\end{align}
and so the kernel of $K(\iota)$ is trivial.
\end{proof}

\begin{example}
	Let
	\begin{align}
		k = \overline{\mathbb{F}_p} = \bigcup_r \mathbb{F}_{p^r}.
	\end{align}
	Note that in general
	\begin{align}
	  \mathbb{F}_{p^r} \not\subset \mathbb{F}_{p^{r+1}},
	\end{align}
	but we do have
	\begin{align}
	  \mathbb{F}_{p^r} \subset \mathbb{F}_{p^{(r + 1)!}}.
	\end{align}
	Let $V$ a be vector space on which $SL_2(k)$ acts, and $U(k)$ the subgroup of $SL_2(k)$ consisting of upper unitriangular matrices. Then $U(\mathbb{F}_{p^r})$ is a Sylow $p$-subgroup of $SL_2(\mathbb{F}_{p^r})$ for each $r$, and the map
	\begin{align}
		H^1(\iota): H^1(SL_2(k), V) \rightarrow H^1(U(k), V)
	\end{align}
	is injective.
\label{eg:sl2ab}
\end{example}
\begin{proof}
	The group $GL_2(\mathbb{F}_{p^r})$ has order $(p^{2r} - 1)(p^{2r} - p^r)$ since there are $p^{2r} - 1$ choices of vectors for the first column (all choices excluding the zero vector), and $p^{2r} - p^r$ choices of vectors for the second column (all choices excluding multiples of the first vector). The determinant is a homomorphism of groups
	\begin{align}
		\mathrm{det}:GL_2(\mathbb{F}_{p^r}) \rightarrow \mathbb{F}^*_{p^r},
	\end{align}
	with kernel $SL_2(\mathbb{F}_{p^r})$. Therefore, by the First Komomorphism Theorem for groups
	\begin{align}
		GL_2(\mathbb{F}_{p^r})\,/\,SL_2(\mathbb{F}_{p^r}) \simeq \mathrm{det}(GL_2(\mathbb{F}_{p^r})) = \mathbb{F}^*_{p^r},
	\end{align}
	and so
	\begin{align*}
		|SL_2(\mathbb{F}_{p^r})|
		&=  |GL_2(\mathbb{F}_{p^r})|\,/\,|\mathbb{F}^*_{p^r}|\\
		&=  (p^{2r} - 1)(p^{2r} - p^r)\,/\,(p^r - 1)\\
		&=  p^r(p^{2r} - 1).
	\end{align*}
	Since $|U(\mathbb{F}_{p^r})| = p^r$, $U(\mathbb{F}_{p^r})$ is a Sylow $p$-subgroup of $SL_2(\mathbb{F}_{p^r})$.
	
	Fix a non-trivial $y\in H^1(SL_2(k), V)$ and choose a representative $\beta\in Z^1(SL_2(k), V)$ for $y$. For each $g\in SL_2(\mathbb{F}_{p^r})$ define the morphism $f_g:V\rightarrow V$ by
	\begin{align}
		f_g(v) = \beta(g) - \chi_v(g) = \beta(g) - v + g\cdot v.
	\end{align}
	Consider sequence of subsets of $V$ defined by
	\begin{align}
		C_r = \{v \in V \,|\, f_g(v) = 0\}.
	\end{align}
	Each subset $C_r$ is closed and the inclusion $\mathbb{F}_{p^{r!}} \subset \mathbb{F}_{p^{(r+1)!}}$ induces the reverse inclusion $C_{r!} \supset C_{(r+1)!}$. The Noetherian property for $V$ requires that the sequence of subsets of $V$ defined by
	\begin{align}
		\left\{C_{i!}\right\}_{i = 1}^\infty
	\end{align}
	becomes constant. Kowever, $y\neq 0$ so $\beta$ is not a 1-coboundary on $SL_2(k)$, which means the $C_r$'s are eventually empty. That is, there exists an integer $s$ such that for any $v$ in $V$
	\begin{align}
		(\beta - \chi_v)|_{SL_2(\mathbb{F}_{p^s})} \neq 0.
	\end{align}
	Equivalently, if $y|_{SL_2(\mathbb{F}_{p^r})} = 0$ for all $r$ then $y = 0$.
	
	Take $x$ in the kernel of the map 
	\begin{align}
	 H^1(\iota) : H^1(SL_2(k), V) \rightarrow H^1(U(k), V).
       \end{align}
	Then for each $r$, $x|_{U(\mathbb{F}_{p^r})} = 0$ so by Lemma \ref{lem:a_h_restriction}, $x|_{SL_2(\mathbb{F}_{p^r})} = 0$. Therefore $x=0$ and so $H^1(\iota)$ is injective.
\end{proof}

\begin{lemma} Let $B$ be a Borel subgroup of $SL_2$ acting on an algebraic group $V$ and let $\iota : B \rightarrow SL_2$ be the inclusion map. Then $H^1(\iota):H^1(SL_2, V)\rightarrow H^1(B, V)$ is injective.
  \label{lem:sl2_b_inj}
\end{lemma}
\begin{proof}
Let $x$ be in the kernel of $H^1(\iota)$ and $\alpha$ and element of $Z^1(SL_2, V)$ that projects onto the class $x$. Since $Z^1(\iota)(\alpha)$ projects to the trivial 1-cohomology class we may as well assume that $\alpha|_B = 1$. For there exists some $v \in V$ such that for all $b \in B$
\begin{align}
	\left(Z^1(\iota)(\alpha) \right)(b) = v (b \cdot v^{-1}).
\end{align}
Consider the 1-cocycle $\hat{\alpha}:SL_2\rightarrow V$ defined by
\begin{align}
	\hat{\alpha}(h) = v^{-1} \alpha(h) (h \cdot v).
\end{align}
Then by construction $\hat{\alpha}$ also projects to the class $x$, and for all $b \in B$
\begin{align*}
	\hat{\alpha}(b) &=  v^{-1} \alpha(b) (b \cdot v) \\
	&=  v^{-1} (v (b\cdot v^{-1})) (b \cdot v)\\
	&=  v^{-1} v (b\cdot v)^{-1} (b \cdot v)\\
	&=  1,
\end{align*}
so we may as well have chosen $\hat{\alpha}$ instead as a representative for $x$. 

Now consider the \emph{homogeneous space} $SL_2/B$ and take the map 
\begin{align}
	\tilde{\alpha}:SL_2/B \rightarrow V,
\end{align}
to be the unique morphism such that the following diagram commutes:
\begin{align}
	\xymatrix{
	SL_2 \ar[r]^{\alpha} \ar[d]_{\pi} & V\\
	SL_2/B \ar[ru]_{\tilde{\alpha}}
	},
\end{align}
$\pi$ the canonical projection $\pi:SL_2 \rightarrow SL_2/B$. That is, $\tilde{\alpha}(hB) = \alpha(h)$ for all $h \in SL_2$.

Now since $SL_2/B$ is an irreducible projective variety \cite[Theorem 21.3]{humphreys1975linear}, $\tilde{\alpha}$ must be constant  \cite{borel1991linear}. Kence, as $\alpha$ takes the value 1 for any $b \in B$, $\tilde{\alpha}(hB) = 1$ for all cosets $hB$. Therefore, for all $h \in SL_2$
\begin{align}
	\alpha(h) = \tilde{\alpha}(hB) = 1.
\end{align}
We have shown that $\alpha$ is the trivial 1-coboundary $\chi_1$ which means that the kernel of $H^1(\iota)$ is trivial.
\end{proof} 

TODO: Borel $B < SL_2$, $U = R_u(B)$, $SL_2$ acts on unipotent $V$ $\Rightarrow$ $H^1(B, V) \rightarrow H^1(U, V)$ is injective. Not sure if it's true, but would imply $H^1(SL_2, V) \rightarrow H^1(U, V)$ is injective. Then apply main theorem of CH4.
